GoLean/GoCore.lean
@@ -2,6 +2,7 @@ import GoLean.GoCore.FloatBits
 import GoLean.GoCore.Machine
 import GoLean.GoCore.StateWf
 import GoLean.GoCore.StepFn
+import GoLean.GoCore.Race
 import GoLean.GoCore.Multi
 import GoLean.GoCore.MachineSound
 import GoLean.GoCore.MultiSound
